{
    "@context": {
        "owl": "http://www.w3.org/2002/07/owl#",
        "rdf": "http://www.w3.org/1999/02/22-rdf-syntax-ns#",
        "rdfs": "http://www.w3.org/2000/01/rdf-schema#",
        "schema": "https://schema.org/",
        "xsd": "http://www.w3.org/2001/XMLSchema#",
        "aiao": "http://purl.org/aiaontology#"
    },
    "@graph": [

        {
            "@id": "aiao:description",
            "@type": "rdf:Property",
            "rdfs:comment": "A textual, human-friendly description of a thing.",
            "rdfs:label": "description",
            "schema:domainIncludes": [
                {
                    "@id": "aiao:Thing"
                }
            ],
            "schema:rangeIncludes": [
                {
                    "@id": "schema:Text"
                }
            ]   
        },

        {
            "@id": "aiao:attributes",
            "@type": "rdf:Property",
            "rdfs:comment": "A list of qualities or features of a thing that can be used, whether independently or in conjunction with other attributes, to identify it.",
            "rdfs:label": "attributes",
            "rdfs:subClassOf": {
                "@id": "schema:ItemList"
            },
            "schema:domainIncludes": [
                {
                    "@id": "aiao:Thing"
                }
            ],
            "schema:rangeIncludes": [
                {
                    "@id": "schema:Attribute"
                }
            ]   
        },

        {
            "@id": "aiao:value",
            "@type": "rdf:Property",
            "rdfs:comment": "The value of an identifier, classifier, parameter or indicator at a specific point in time.",
            "rdfs:label": "value",
            "schema:domainIncludes": [
                {
                    "@id": "aiao:Classification"
                },
                {
                    "@id": "aiao:Identification"
                },
                {
                    "@id": "aiao:State"
                }
            ],
            "schema:rangeIncludes": [
                {
                    "@id": "schema:Text"
                },
                {
                    "@id": "schema:Number"
                },
                {
                    "@id": "schema:Boolean"
                }
            ]   
        },
        
        {
            "@id": "aiao:claimant",
            "@type": "rdf:Property",
            "rdfs:comment": "The agent who is making the claim.",
            "rdfs:label": "claimant",
            "schema:domainIncludes": [
                {
                    "@id": "aiao:Claim"
                }
            ],
            "schema:rangeIncludes": [
                {
                    "@id": "schema:Text"
                },
                {
                    "@id": "aiao:Agent"
                }
            ]   
        },
        
        {
            "@id": "aiao:substantiations",
            "@type": "rdf:Property",
            "rdfs:comment": "A list of things, or references to things, presented in support of a specific claim.",
            "rdfs:label": "substantiations",
            "rdfs:subClassOf": {
                "@id": "schema:ItemList"
            },
            "schema:domainIncludes": [
                {
                    "@id": "aiao:Claim"
                }
            ],
            "schema:rangeIncludes": [
                {
                    "@id": "schema:Text"
                },
                {
                    "@id": "aiao:Thing"
                }
            ]
        },

        {
            "@id": "aiao:identifier",
            "@type": "rdf:Property",
            "rdfs:comment": "An identification system.",
            "rdfs:label": "identifier",
            "schema:domainIncludes": [
                {
                    "@id": "aiao:Identification"
                }
            ],
            "schema:rangeIncludes": [
                {
                    "@id": "aiao:IdentificationSystem"
                }
            ]
        },

        {
            "@id": "aiao:identifications",
            "@type": "rdf:Property",
            "rdfs:comment": "A list of identifications for a thing.",
            "rdfs:label": "identifications",
            "rdfs:subClassOf": {
                "@id": "schema:ItemList"
            },
            "schema:domainIncludes": [
                {
                    "@id": "aiao:Thing"
                }
            ],
            "schema:rangeIncludes": [
                {
                    "@id": "aiao:Identification"
                }
            ]
        },

        {
            "@id": "aiao:classifier",
            "@type": "rdf:Property",
            "rdfs:comment": "A classification system.",
            "rdfs:label": "classifier",
            "schema:domainIncludes": [
                {
                    "@id": "aiao:Classification"
                }
            ],
            "schema:rangeIncludes": [
                {
                    "@id": "aiao:ClassificationSystem"
                }
            ]
        },

        {
            "@id": "aiao:classifications",
            "@type": "rdf:Property",
            "rdfs:comment": "A list of classifications of a thing.",
            "rdfs:label": "classifications",
            "rdfs:subClassOf": {
                "@id": "schema:ItemList"
            },
            "schema:domainIncludes": [
                {
                    "@id": "aiao:Thing"
                }
            ],
            "schema:rangeIncludes": [
                {
                    "@id": "aiao:Classification"
                }
            ]
        },

        {
            "@id": "aiao:parameters",
            "@type": "rdf:Property",
            "rdfs:comment": "A list of parameters defining a particular scope or extent of a thing.",
            "rdfs:label": "parameters",
            "rdfs:subClassOf": {
                "@id": "schema:ItemList"
            },
            "schema:domainIncludes": [
                {
                    "@id": "aiao:Thing"
                }
            ],
            "schema:rangeIncludes": [
                {
                    "@id": "schema:Parameter"
                }
            ]
        },

        {
            "@id": "aiao:temporalExtent",
            "@type": "rdf:Property",
            "rdfs:comment": "The temporal extent of a thing, expressed as a period or duration.",
            "rdfs:label": "temporalExtent",
            "rdfs:subClassOf": {
                "@id": "aiao:TemporalParameter"
            },
            "schema:domainIncludes": [
                {
                    "@id": "aiao:Thing"
                }
            ],
            "schema:rangeIncludes": [
                {
                    "@id": "aiao:Period"
                },
                {
                    "@id": "aiao:Duration"
                }
            ]
        },

        {
            "@id": "aiao:spatialExtent",
            "@type": "rdf:Property",
            "rdfs:comment": "The spatial extent of a thing, expressed as a line (one dimension), area (two dimensions) or volume (three dimensions).",
            "rdfs:label": "substantiations",
            "rdfs:subClassOf": {
                "@id": "aiao:SpatialParameter"
            },
            "schema:domainIncludes": [
                {
                    "@id": "aiao:Thing"
                }
            ],
            "schema:rangeIncludes": [
                {
                    "@id": "aiao:Line"
                },
                {
                    "@id": "aiao:Area"
                },
                {
                    "@id": "aiao:Volume"
                }
            ]
        },

        {
            "@id": "aiao:temporalLocation",
            "@type": "rdf:Property",
            "rdfs:comment": "The temporal location of a thing, expressed as a period or duration.",
            "rdfs:label": "temporalExtent",
            "rdfs:subClassOf": {
                "@id": "aiao:TemporalParameter"
            },
            "schema:domainIncludes": [
                {
                    "@id": "aiao:Thing"
                }
            ],
            "schema:rangeIncludes": [
                {
                    "@id": "aiao:Period"
                },
                {
                    "@id": "aiao:Duration"
                }
            ]
        },

        {
            "@id": "aiao:controls",
            "@type": "rdf:Property",
            "rdfs:comment": "The controls (whether binding or non-binding) that limit or guide a thing.",
            "rdfs:label": "controls",
            "rdfs:subClassOf": {
                "@id": "schema:ItemList"
            },
            "schema:domainIncludes": [
                {
                    "@id": "aiao:Thing"
                }
            ],
            "schema:rangeIncludes": [
                {
                    "@id": "aiao:Control"
                }
            ]
        },

        {
            "@id": "aiao:activities",
            "@type": "rdf:Property",
            "rdfs:comment": "The activities that an event comprises.",
            "rdfs:label": "activities",
            "rdfs:subClassOf": {
                "@id": "schema:ItemList"
            },
            "schema:domainIncludes": [
                {
                    "@id": "aiao:Thing"
                }
            ],
            "schema:rangeIncludes": [
                {
                    "@id": "aiao:Activity"
                }
            ]
        },

        {
            "@id": "aiao:subject",
            "@type": "rdf:Property",
            "rdfs:comment": "The thing in question. As a property of aiao:Claim it is the thing about which the claim is being made; as a property of aiao:State it is the thing of which the state is being describe; as a property of aiao:StateChange it is the thing that underwent a state change.",
            "rdfs:label": ["subject", "activity", "agent"],
            "schema:domainIncludes": [
                {
                    "@id": "aiao:Claim"
                },
                {
                    "@id": "aiao:State"
                },
                {
                    "@id": "aiao:StateChange"
                }
            ],
            "schema:rangeIncludes": [
                {
                    "@id": "aiao:Thing"
                }
            ]
        },

        {
            "@id": "aiao:provenance",
            "@type": "rdf:Property",
            "rdfs:comment": "The cause of the thing in question. Must be an event or an activity.",
            "rdfs:label": "provenance",
            "schema:domainIncludes": [
                {
                    "@id": "aiao:Thing"
                }
            ],
            "schema:rangeIncludes": [
                {
                    "@id": "aiao:Event"
                }
            ]
        },

        {
            "@id": "aiao:superinstance",
            "@type": "rdf:Property",
            "rdfs:comment": "The encompassing instance, if any, of a thing. Must be of the same class as the thing itself, or one of the superclasses thereof.",
            "rdfs:label": "superinstance",
            "schema:domainIncludes": [
                {
                    "@id": "aiao:Thing"
                }
            ],
            "schema:rangeIncludes": [
                {
                    "@id": "aiao:Thing"
                }
            ]
        },

        {
            "@id": "aiao:subinstances",
            "@type": "rdf:Property",
            "rdfs:comment": "The instances, if any, that are encompassed by the thing in question. Must be of the same class as the thing itself, or one of the subclasses thereof.",
            "rdfs:label": "things",
            "rdfs:subClassOf": {
                "@id": "schema:ItemList"
            },
            "schema:domainIncludes": [
                {
                    "@id": "aiao:Thing"
                }
            ],
            "schema:rangeIncludes": [
                {
                    "@id": "aiao:Thing"
                }
            ]
        }
    ]  
}
